make modular reduction work for a < r * r

code/bignum/Hacl.Bignum.ModReduction.fst
@@ -17,57 +17,38 @@ module B = LowStar.Buffer
 module S = Hacl.Spec.Bignum.ModReduction
 module BN = Hacl.Bignum
 module BM = Hacl.Bignum.Montgomery
+module BAM = Hacl.Bignum.AlmostMontgomery
 
 #reset-options "--z3rlimit 50 --fuel 0 --ifuel 0"
 
 inline_for_extraction noextract
-let bn_check_mod_st (t:limb_t) (len:BN.meta_len t) =
-    n:lbignum t len
-  -> a:lbignum t (len +! len) ->
-  Stack (limb t)
-  (requires fun h -> live h n /\ live h a)
-  (ensures  fun h0 r h1 -> modifies0 h0 h1 /\
-    r == S.bn_check_mod (as_seq h0 n) (as_seq h0 a))
-
-
-inline_for_extraction noextract
-val bn_check_mod: #t:limb_t -> k:BM.mont t -> bn_check_mod_st t k.BM.bn.BN.len
-let bn_check_mod #t k n a =
-  [@inline_let] let len = k.BM.bn.BN.len in
-  push_frame ();
-  let m0 = BM.mont_check n in
-  let n2 = create (len +! len) (uint #t #SEC 0) in
-  BN.mul n n n2;
-  let m1 = BN.bn_lt_mask (len +! len) a n2 in
-  let r = m0 &. m1 in
-  pop_frame ();
-  r
-
-
-inline_for_extraction noextract
 let bn_mod_slow_precompr2_st (t:limb_t) (len:BN.meta_len t) =
-    n:lbignum t len
-  -> a:lbignum t (len +! len)
+     n:lbignum t len
+  -> mu:limb t
   -> r2:lbignum t len
+  -> a:lbignum t (len +! len)
   -> res:lbignum t len ->
   Stack unit
   (requires fun h ->
     live h n /\ live h a /\ live h r2 /\ live h res /\
     disjoint res n /\ disjoint res a /\ disjoint res r2 /\ disjoint r2 n)
   (ensures  fun h0 _ h1 -> modifies (loc res) h0 h1 /\
-    as_seq h1 res == S.bn_mod_slow_precompr2 (as_seq h0 n) (as_seq h0 a) (as_seq h0 r2))
+    as_seq h1 res == S.bn_mod_slow_precompr2 (as_seq h0 n) mu (as_seq h0 r2) (as_seq h0 a))
 
 
 inline_for_extraction noextract
-val bn_mod_slow_precompr2: #t:limb_t -> k:BM.mont t -> bn_mod_slow_precompr2_st t k.BM.bn.BN.len
-let bn_mod_slow_precompr2 #t k n a r2 res =
+val bn_mod_slow_precompr2:
+    #t:limb_t
+  -> k:BM.mont t ->
+  bn_mod_slow_precompr2_st t k.BM.bn.BN.len
+
+let bn_mod_slow_precompr2 #t k n mu r2 a res =
   [@inline_let] let len = k.BM.bn.BN.len in
   push_frame ();
   let a_mod = create len (uint #t #SEC 0) in
   let a1 = create (len +! len) (uint #t #SEC 0) in
   copy a1 a;
-  let mu = BM.mod_inv_limb n.(0ul) in
-  BM.reduction n mu a1 a_mod;
+  BAM.bn_almost_mont_reduction k.BM.bn n mu a1 a_mod;
   BM.to n mu r2 a_mod res;
   pop_frame ()
 
@@ -96,7 +77,8 @@ val bn_mod_slow:
 let bn_mod_slow #t k bn_mod_slow_precompr2 nBits n a res =
   [@inline_let] let len = k.BM.bn.BN.len in
   push_frame ();
+  let mu = BM.mod_inv_limb n.(0ul) in
   let r2 = create len (uint #t #SEC 0) in
   BM.precomp nBits n r2;
-  bn_mod_slow_precompr2 n a r2 res;
+  bn_mod_slow_precompr2 n mu r2 a res;
   pop_frame ()
